proof/common/Array2464.ec
@@ -1,0 +1,3 @@
+from Jasmin require import JArray.
+
+clone export PolyArray as Array2464  with op size <- 2464.
